Add RA race checking semantics

src/localdrfra/OrdStep.v
@@ -304,22 +304,14 @@ Module OrdConfiguration.
     Variable ordc: Ordering.t.
 
     Inductive step: forall (e: MachineEvent.t) (tid: Ident.t) (c1 c2: Configuration.t), Prop :=
-    | step_failure
-        pf tid c1 lang st1 lc1 e2 st3 lc3 sc3 memory3
-        (TID: IdentMap.find tid c1.(Configuration.threads) = Some (existT _ lang st1, lc1))
-        (STEPS: rtc (@OrdThread.tau_step _ L ordc)
-                    (Thread.mk _ st1 lc1 c1.(Configuration.sc) c1.(Configuration.memory)) e2)
-        (STEP: OrdThread.step L ordc pf ThreadEvent.failure e2 (Thread.mk _ st3 lc3 sc3 memory3)):
-        step MachineEvent.failure tid
-             c1 (Configuration.mk (IdentMap.add tid (existT _ _ st3, lc3) c1.(Configuration.threads)) sc3 memory3)
-    | step_normal
+    | step_intro
         pf e tid c1 lang st1 lc1 e2 st3 lc3 sc3 memory3
         (TID: IdentMap.find tid c1.(Configuration.threads) = Some (existT _ lang st1, lc1))
         (STEPS: rtc (@OrdThread.tau_step _ L ordc)
                     (Thread.mk _ st1 lc1 c1.(Configuration.sc) c1.(Configuration.memory)) e2)
         (STEP: OrdThread.step L ordc pf e e2 (Thread.mk _ st3 lc3 sc3 memory3))
-        (EVENT: e <> ThreadEvent.failure)
-        (CONSISTENT: OrdThread.consistent L ordc (Thread.mk lang st3 lc3 sc3 memory3)):
+        (CONSISTENT: e <> ThreadEvent.failure ->
+                     OrdThread.consistent L ordc (Thread.mk lang st3 lc3 sc3 memory3)):
         step (ThreadEvent.get_machine_event e) tid
              c1 (Configuration.mk (IdentMap.add tid (existT _ _ st3, lc3) c1.(Configuration.threads)) sc3 memory3)
     .
