src/localdrfra/RARace.v
@@ -55,138 +55,178 @@ Module ReleaseWrites.
 End ReleaseWrites.
 
 
-Module RATrace.
-  Section RATrace.
+Module RAThread.
+  Section RAThread.
+    Variable lang: language.
     Variable L: Loc.t -> bool.
 
-    Inductive thread_steps lang: forall (rels: ReleaseWrites.t) (e1 e2: Thread.t lang), Prop :=
-    | thread_steps_refl
+    Definition ra_race (rels: ReleaseWrites.t) (tview: TView.t) (loc: Loc.t) (to: Time.t) (ordr: Ordering.t): Prop :=
+      (<<LOC: L loc>>) /\
+      (<<HIGHER: Time.lt (tview.(TView.cur).(View.rlx) loc) to>>) /\
+      ((<<ORDW: ~ List.In (loc, to) rels>>) \/
+       (<<ORDR: Ordering.le ordr Ordering.strong_relaxed>>)).
+
+    Inductive step rels1: forall (rels2: ReleaseWrites.t) (e: ThreadEvent.t) (e1 e2: Thread.t lang), Prop :=
+    | step_normal
+        pf e e1 e2
+        (STEP: @OrdThread.step lang L Ordering.acqrel pf e e1 e2):
+        step rels1 (ReleaseWrites.append L e rels1) e e1 e2
+    | step_race
+        pf e e1 e2
+        loc to val released ord
+        (STEP: @OrdThread.step lang L Ordering.acqrel pf e e1 e2)
+        (CONS: Local.promise_consistent e1.(Thread.local))
+        (EVENT: ThreadEvent.is_reading e = Some (loc, to, val, released, ord))
+        (RACE: ra_race rels1 e1.(Thread.local).(Local.tview) loc to ord):
+        step rels1 (ReleaseWrites.append L e rels1) ThreadEvent.failure e1 e2
+    .
+
+    Inductive steps rels1: forall (rels2: ReleaseWrites.t) (e1 e2: Thread.t lang), Prop :=
+    | steps_refl
         e:
-        thread_steps lang [] e e
-    | thread_steps_step
-        rels pf e e1 e2 e3
-        (STEPS: @thread_steps lang rels e1 e2)
-        (STEP: @OrdThread.step lang L Ordering.acqrel pf e e2 e3):
-        thread_steps lang (ReleaseWrites.append L e rels) e1 e3
+        steps rels1 rels1 e e
+    | steps_step
+        rels2 rels3 e e1 e2 e3
+        (STEP: step rels1 rels2 e e1 e2)
+        (STEPS: steps rels2 rels3 e2 e3):
+        steps rels1 rels3 e1 e3
     .
-    Hint Constructors thread_steps.
+    Hint Constructors steps.
 
-    Inductive thread_tau_steps lang: forall (rels: ReleaseWrites.t) (e1 e2: Thread.t lang), Prop :=
-    | thread_tau_steps_refl
+    Inductive tau_steps rels1: forall (rels2: ReleaseWrites.t) (e1 e2: Thread.t lang), Prop :=
+    | tau_steps_refl
         e:
-        thread_tau_steps lang [] e e
-    | thread_tau_steps_step
-        rels pf e e1 e2 e3
-        (STEPS: @thread_tau_steps lang rels e1 e2)
-        (STEP: @OrdThread.step lang L Ordering.acqrel pf e e2 e3)
-        (SILENT: ThreadEvent.get_machine_event e = MachineEvent.silent):
-        thread_tau_steps lang (ReleaseWrites.append L e rels) e1 e3
+        tau_steps rels1 rels1 e e
+    | tau_steps_step
+        rels2 rels3 e e1 e2 e3
+        (STEP: step rels1 rels2 e e1 e2)
+        (SILENT: ThreadEvent.get_machine_event e = MachineEvent.silent)
+        (STEPS: tau_steps rels2 rels3 e2 e3):
+        tau_steps rels1 rels3 e1 e3
     .
-    Hint Constructors thread_steps.
+    Hint Constructors tau_steps.
 
-    Inductive configuration_step: forall (e: MachineEvent.t) (tid: Ident.t) (rels: ReleaseWrites.t) (c1 c2: Configuration.t), Prop :=
-    | configuration_step_intro
-        rels
-        pf e tid c1 lang st1 lc1 e2 st3 lc3 sc3 memory3
-        (TID: IdentMap.find tid c1.(Configuration.threads) = Some (existT _ lang st1, lc1))
-        (STEPS: thread_tau_steps lang rels (Thread.mk _ st1 lc1 c1.(Configuration.sc) c1.(Configuration.memory)) e2)
-        (STEP: OrdThread.step L Ordering.acqrel pf e e2 (Thread.mk _ st3 lc3 sc3 memory3))
-        (CONSISTENT: OrdThread.consistent L Ordering.acqrel (Thread.mk _ st3 lc3 sc3 memory3)):
-        configuration_step (ThreadEvent.get_machine_event e) tid (ReleaseWrites.append L e rels)
-                           c1 (Configuration.mk (IdentMap.add tid (existT _ _ st3, lc3) c1.(Configuration.threads)) sc3 memory3)
-    .
-    Hint Constructors configuration_step.
+    Definition steps_failure (rels1: ReleaseWrites.t) (e1: Thread.t lang): Prop :=
+      exists rels2 rels3 e2 e3,
+        (<<STEPS: tau_steps rels1 rels2 e1 e2>>) /\
+        (<<FAILURE: step rels2 rels3 ThreadEvent.failure e2 e3>>).
+    Hint Unfold steps_failure.
 
-    Inductive configuration_steps: forall (rels: ReleaseWrites.t) (c1 c2: Configuration.t), Prop :=
-    | configuration_steps_refl
-        c:
-        configuration_steps [] c c
-    | configuration_steps_step
-        rels e tid rels' c1 c2 c3
-        (STEPS: configuration_steps rels c1 c2)
-        (STEP: configuration_step e tid rels' c2 c3):
-        configuration_steps (rels' ++ rels) c1 c3
-    .
-    Hint Constructors configuration_steps.
+    Definition consistent (rels: ReleaseWrites.t) (e: Thread.t lang): Prop :=
+      forall mem1 sc1
+        (CAP: Memory.cap e.(Thread.memory) mem1)
+        (SC_MAX: Memory.max_concrete_timemap mem1 sc1),
+        (<<FAILURE: steps_failure rels (Thread.mk lang e.(Thread.state) e.(Thread.local) sc1 mem1)>>) \/
+        exists rels2 e2,
+          <<STEPS: tau_steps rels rels2 (Thread.mk lang e.(Thread.state) e.(Thread.local) sc1 mem1) e2>> /\
+          <<PROMISES: e2.(Thread.local).(Local.promises) = Memory.bot>>.
 
-    Lemma thread_tau_steps_steps
-          lang rels e1 e2
-          (STEPS: thread_tau_steps lang rels e1 e2):
-      thread_steps lang rels e1 e2.
+
+    Lemma tau_steps_steps
+          rels1 rels2 e1 e2
+          (STEPS: tau_steps rels1 rels2 e1 e2):
+      steps rels1 rels2 e1 e2.
     Proof.
       induction STEPS; eauto.
     Qed.
 
-    Lemma thread_steps_app
-          lang rels1 rels2 e1 e2 e3
-          (STEPS1: thread_steps lang rels1 e1 e2)
-          (STEPS2: thread_steps lang rels2 e2 e3):
-      thread_steps lang (rels2 ++ rels1) e1 e3.
+    Lemma steps_app
+          rels1 rels2 rels3 e1 e2 e3
+          (STEPS1: steps rels1 rels2 e1 e2)
+          (STEPS2: steps rels2 rels3 e2 e3):
+      steps rels1 rels3 e1 e3.
     Proof.
-      revert rels1 e1 STEPS1. induction STEPS2; i; eauto.
-      exploit IHSTEPS2; eauto. i.
-      rewrite ReleaseWrites.append_app. econs 2; eauto.
+      revert rels3 e3 STEPS2.
+      induction STEPS1; i; eauto.
     Qed.
 
-    Lemma thread_tau_steps_app
-          lang rels1 rels2 e1 e2 e3
-          (STEPS1: thread_tau_steps lang rels1 e1 e2)
-          (STEPS2: thread_tau_steps lang rels2 e2 e3):
-      thread_tau_steps lang (rels2 ++ rels1) e1 e3.
+    Lemma tau_steps_app
+          rels1 rels2 rels3 e1 e2 e3
+          (STEPS1: tau_steps rels1 rels2 e1 e2)
+          (STEPS2: tau_steps rels2 rels3 e2 e3):
+      tau_steps rels1 rels3 e1 e3.
     Proof.
-      revert rels1 e1 STEPS1. induction STEPS2; i; eauto.
-      exploit IHSTEPS2; eauto. i.
-      rewrite ReleaseWrites.append_app. econs 2; eauto.
+      revert rels3 e3 STEPS2.
+      induction STEPS1; i; eauto.
     Qed.
 
-    Lemma thread_tau_steps_rtc_tau_step
-          lang rels e1 e2
-          (STEPS: thread_tau_steps lang rels e1 e2):
+    Lemma tau_steps_rtc_tau_step
+          rels1 rels2 e1 e2
+          (STEPS: tau_steps rels1 rels2 e1 e2):
       rtc (@OrdThread.tau_step lang L Ordering.acqrel) e1 e2.
     Proof.
       induction STEPS; eauto.
-      exploit rtc_n1; try exact IHSTEPS; eauto.
+      econs 2; eauto. inv STEP; ss.
       econs; eauto. econs. eauto.
     Qed.
+  End RAThread.
+End RAThread.
 
-    Lemma configuration_step_ord_step
-          e tid rels c1 c2
-          (STEP: configuration_step e tid rels c1 c2):
-      OrdConfiguration.step L Ordering.acqrel e tid c1 c2.
-    Proof.
-      inv STEP. exploit thread_tau_steps_rtc_tau_step; eauto. i.
-      destruct (ThreadEvent.get_machine_event e0) eqn:EVENT.
-      - rewrite <- EVENT. econs 2; eauto. destruct e0; ss.
-      - rewrite <- EVENT. econs 2; eauto. destruct e0; ss.
-      - destruct e0; ss. econs 1; eauto.
-    Qed.
-  End RATrace.
-End RATrace.
+
+Module RAConfiguration.
+  Section RAConfiguration.
+    Variable L: Loc.t -> bool.
+
+    Inductive step:
+      forall (e: MachineEvent.t) (tid: Ident.t) (rels1 rels2: ReleaseWrites.t) (c1 c2: Configuration.t), Prop :=
+    | step_intro
+        rels1 rels2 rels3
+        e tid c1 lang st1 lc1 e2 st3 lc3 sc3 memory3
+        (TID: IdentMap.find tid c1.(Configuration.threads) = Some (existT _ lang st1, lc1))
+        (STEPS: RAThread.tau_steps lang L rels1 rels2
+                                   (Thread.mk _ st1 lc1 c1.(Configuration.sc) c1.(Configuration.memory)) e2)
+        (STEP: RAThread.step lang L rels2 rels3 e e2 (Thread.mk _ st3 lc3 sc3 memory3))
+        (CONSISTENT: e <> ThreadEvent.failure ->
+                     RAThread.consistent lang L rels3 (Thread.mk _ st3 lc3 sc3 memory3)):
+        step (ThreadEvent.get_machine_event e) tid rels1 rels3
+             c1 (Configuration.mk (IdentMap.add tid (existT _ _ st3, lc3) c1.(Configuration.threads)) sc3 memory3)
+    .
+
+    Inductive steps rels1: forall (rels2: ReleaseWrites.t) (c1 c2: Configuration.t), Prop :=
+    | steps_refl
+        c:
+        steps rels1 rels1 c c
+    | steps_step
+        rels2 rels3 e tid c1 c2 c3
+        (STEP: step e tid rels1 rels2 c1 c2)
+        (STEPS: steps rels2 rels3 c2 c3):
+        steps rels1 rels3 c1 c3
+    .
+    Hint Constructors steps.
+
+    (* Lemma step_ord_step *)
+    (*       e tid rels1 rels2 c1 c2 *)
+    (*       (STEP: step e tid rels1 rels2 c1 c2): *)
+    (*   OrdConfiguration.step L Ordering.acqrel e tid c1 c2. *)
+    (* Proof. *)
+    (*   inv STEP. exploit RAThread.tau_steps_rtc_tau_step; eauto. i. *)
+    (*   econs; eauto. *)
+    (*   destruct (ThreadEvent.get_machine_event e0) eqn:EVENT. *)
+    (*   - rewrite <- EVENT. econs 2; eauto. destruct e0; ss. *)
+    (*   - rewrite <- EVENT. econs 2; eauto. destruct e0; ss. *)
+    (*   - destruct e0; ss. econs 1; eauto. *)
+    (* Qed. *)
+  End RAConfiguration.
+End RAConfiguration.
 
 
 Module RARace.
   Section RARace.
     Variable L: Loc.t -> bool.
 
-    Definition ra_race (rels: ReleaseWrites.t) (tview: TView.t) (loc: Loc.t) (to: Time.t) (ordr: Ordering.t): Prop :=
-      <<LOC: L loc>> /\
-      <<HIGHER: Time.lt (tview.(TView.cur).(View.rlx) loc) to>> /\
-      (<<ORDW: ~ List.In (loc, to) rels>> \/
-       <<ORDR: Ordering.le ordr Ordering.strong_relaxed>>).
-
-    Definition racefree (s: Threads.syntax): Prop :=
-      forall rels1 c
-        tid lang st1 lc1
-        rels2 pf e loc to val released ord e2 e3
-        (CSTEPS: RATrace.configuration_steps L rels1 (Configuration.init s) c)
-        (TID: IdentMap.find tid c.(Configuration.threads) = Some (existT _ lang st1, lc1))
-        (STEPS: RATrace.thread_steps L lang rels2
-                                     (Thread.mk _ st1 lc1 c.(Configuration.sc) c.(Configuration.memory))
-                                     e2)
-        (CONS: Local.promise_consistent e2.(Thread.local))
-        (STEP: OrdThread.step L Ordering.acqrel pf e e2 e3)
-        (READ: ThreadEvent.is_reading e = Some (loc, to, val, released, ord))
-        (RACE: ra_race (rels2 ++ rels1) e2.(Thread.local).(Local.tview) loc to ord),
-        False.
+    (* Definition racefree (s: Threads.syntax): Prop := *)
+    (*   forall rels1 c *)
+    (*     tid lang st1 lc1 *)
+    (*     rels2 pf e loc to val released ord e2 e3 *)
+    (*     (CSTEPS: RATrace.configuration_steps L rels1 (Configuration.init s) c) *)
+    (*     (TID: IdentMap.find tid c.(Configuration.threads) = Some (existT _ lang st1, lc1)) *)
+    (*     (STEPS: RATrace.thread_steps L lang rels2 *)
+    (*                                  (Thread.mk _ st1 lc1 c.(Configuration.sc) c.(Configuration.memory)) *)
+    (*                                  e2) *)
+    (*     (CONS: Local.promise_consistent e2.(Thread.local)) *)
+    (*     (STEP: OrdThread.step L Ordering.acqrel pf e e2 e3) *)
+    (*     (READ: ThreadEvent.is_reading e = Some (loc, to, val, released, ord)) *)
+    (*     (RACE: ra_race (rels2 ++ rels1) e2.(Thread.local).(Local.tview) loc to ord), *)
+    (*     False. *)
   End RARace.
 End RARace.
